\documentclass[10pt]{article}

\renewcommand{\d}{\mathrm{d}}
\renewcommand{\(}{\left(}
\renewcommand{\)}{\right)}


\begin{document}
\section{Problem}
Prove that
\[
\int\limits_{0}^{1}
\frac{\ln t\ \d t}{1+t} = -\frac{\pi^2}{12}.
\]

\section{Solution}
\subsection{Step 1.}
Consider the function
\[
F(x) = \int\limits_{0}^{1}
\frac{x\ln t\ \d t}{x+t}.
\]
Taking derivative in $x$, we find that
\[F'(x) = -\frac{\ln (1+x)}{x},\]
and hence
\begin{equation}\label{F}
F(x)=-\int\limits_0^{x}\frac{\ln(1+t)\,\d t}{t}.
\end{equation}
\textbf{Proof.}
Indeed,
\[
F'(x) = \int\limits_{0}^{1}
\frac{\ln t\ \d t}{x+t}
-
\int\limits_{0}^{1}
\frac{x\ln t\ \d t}{(x+t)^2}
=
\int\limits_{0}^{1}
\frac{t\ln t\ \d t}{(x+t)^2}.
\]
Integrating here by parts, we find
\[
\int\limits_{0}^{1}
\frac{t\ln t\ \d t}{(x+t)^2}
=
\int\limits_{0}^{1}\partial_t\(\frac{-1}{x+t}\)
\cdot t\ln t\ \d t
=
-\frac{t\ln t}{(x+t)}\Big|_{t=0}^{t=1}+
\int\limits_0^1\frac{(\ln t + 1)\d t}{x+t}
=.
\]
where in the second integral we integrated by parts.

\noindent\textbf{End of proof. }\hfill$\triangle$
\subsection{Step 2.}
Expanding the logarithm into series
\[\ln (1+t)=\sum\limits_{j=0}^{\infty}\frac{(-1)^{j-1}t^{j}}{j}\]

\end{document}